theories/theories/utp_designs_a.thy
@@ -1,0 +1,69 @@
+theory utp_designs_a
+imports utp_designs
+begin
+
+lift_definition DesignA :: 
+  "'a WF_ALPHA_PREDICATE \<Rightarrow> 
+   'a WF_ALPHA_PREDICATE \<Rightarrow> 
+   'a WF_ALPHA_PREDICATE" (infixr "\<turnstile>\<^sub>\<alpha>" 60)
+is "\<lambda> P Q. (\<alpha> P \<union>\<^sub>f \<alpha> Q \<union>\<^sub>f \<lbrace>okay\<down>, okay\<down>\<acute>\<rbrace>, (\<pi> P) \<turnstile> (\<pi> Q))"
+  apply (simp add:WF_ALPHA_PREDICATE_def WF_PREDICATE_OVER_def)
+  apply (auto intro:unrest)
+done
+
+lemma REL_ALPHABET_in_alpha [closure]: "in\<^sub>\<alpha>a \<in> REL_ALPHABET"
+  by (auto simp add:REL_ALPHABET_def var_defs)
+
+
+lemma REL_ALPHABET_out_alpha [closure]: "out\<^sub>\<alpha>a \<in> REL_ALPHABET"
+  by (auto simp add:REL_ALPHABET_def var_defs)
+
+
+lemma DesignA_alphabet [alphabet]:
+  "\<alpha> (P \<turnstile>\<^sub>\<alpha> Q) = \<alpha> P \<union>\<^sub>f \<alpha> Q \<union>\<^sub>f \<lbrace>okay\<down>, okay\<down>\<acute>\<rbrace>"
+  by (simp add:DesignA.rep_eq pred_alphabet_def)
+
+lemma DesignA_evala [evala]:
+  "\<lbrakk>P \<turnstile>\<^sub>\<alpha> Q\<rbrakk>\<pi> = \<lbrakk>P\<rbrakk>\<pi> \<turnstile> \<lbrakk>Q\<rbrakk>\<pi>"
+  by (simp add:EvalA_def DesignA.rep_eq)
+
+lemma DesignA_rel_closure [closure]:
+  "\<lbrakk> P \<in> WF_ALPHA_REL; Q \<in> WF_ALPHA_REL \<rbrakk> \<Longrightarrow> P \<turnstile>\<^sub>\<alpha> Q \<in> WF_ALPHA_REL"
+  apply (simp add:WF_ALPHA_REL_def REL_ALPHABET_def alphabet)
+  apply (simp add:closure)
+done
+
+lemma WF_ALPHA_REL_EvalA_WF_RELATION [closure]:
+  "P \<in> WF_ALPHA_REL \<Longrightarrow> \<lbrakk>P\<rbrakk>\<pi> \<in> WF_RELATION"
+  apply (simp add:WF_ALPHA_REL_def WF_RELATION_def REL_ALPHABET_def)
+  apply (rule UNREST_subset)
+  apply (rule unrest) back back back
+  apply (auto)
+done
+
+lemma UNREST_OKAY_alpha [unrest]: "\<lbrakk> okay\<down> \<notin>\<^sub>f \<alpha> P; okay\<down>\<acute> \<notin>\<^sub>f \<alpha> P \<rbrakk> \<Longrightarrow> OKAY \<sharp> \<lbrakk>P\<rbrakk>\<pi>"
+  apply (rule UNREST_subset)
+  apply (rule EvalA_UNREST)
+  apply (auto)
+done
+
+theorem DesignA_composition:
+  assumes 
+  "P1 \<in> WF_ALPHA_REL" "P2 \<in> WF_ALPHA_REL"
+  "Q1 \<in> WF_ALPHA_REL" "Q2 \<in> WF_ALPHA_REL"
+  "okay\<down> \<notin>\<^sub>f \<alpha> P1" "okay\<down>\<acute> \<notin>\<^sub>f \<alpha> P1"
+  "okay\<down> \<notin>\<^sub>f \<alpha> P2" "okay\<down>\<acute> \<notin>\<^sub>f \<alpha> P2"
+  "okay\<down> \<notin>\<^sub>f \<alpha> Q1" "okay\<down>\<acute> \<notin>\<^sub>f \<alpha> Q1"
+  "okay\<down> \<notin>\<^sub>f \<alpha> Q2" "okay\<down>\<acute> \<notin>\<^sub>f \<alpha> Q2"
+  shows "(P1 \<turnstile>\<^sub>\<alpha> Q1) ;\<^sub>\<alpha> (P2 \<turnstile>\<^sub>\<alpha> Q2) = ((\<not>\<^sub>\<alpha> ((\<not>\<^sub>\<alpha> P1) ;\<^sub>\<alpha> true\<^bsub>in\<^sub>\<alpha> (\<alpha> P1)\<^esub>)) \<and>\<^sub>\<alpha> \<not>\<^sub>\<alpha> (Q1 ;\<^sub>\<alpha> (\<not>\<^sub>\<alpha> P2))) \<turnstile>\<^sub>\<alpha> (Q1 ;\<^sub>\<alpha> Q2)"
+  using assms
+  apply (utp_alpha_tac)
+  apply (rule conjI)
+  apply (simp add:alphabet_dist closure)
+  defer
+  apply (subst DesignD_composition)
+  apply (simp_all add:closure unrest)
+  apply (auto)[1]
+done
+
+end
